adding notion of relabeling

src/Rdf.v
@@ -1,53 +1,73 @@
-From Coq Require Import Lists.ListSet.
-From Coq Require Import Init.Nat.
-From Coq Require Import Strings.String.
-From Coq Require Import Bool.Bool.
+From mathcomp Require Import all_ssreflect.
+Set Implicit Arguments.
+Unset Strict Implicit.
+Unset Printing Implicit Defensive.
 From RDF Require Import Term.
-From RDF Require Import Maps.
+(* From RDF Require Import Maps. *)
 From RDF Require Import Triple.
 
+Section rdf.
+  Variable I B L: eqType.
+  Let term:= (term I B L).
+  Let triple:= (triple I B L).
 
-(* Not sure if its a good idea to have a set, 
- may be we want some order on the triples *)
-Record rdf_graph := mkRdfGraph
-  {
-    graph : set trpl
-    (* subject_in_IL : forall t in rdf_graph,   *)
-    (* predicate_in_I : forall t in rdf_graph,   *)
-    (* object_in_IBL : forall t in rdf_graph,   *)
+  Record rdf_graph := mkRdfGraph {
+                         graph : seq triple
+                       ; subject_in_IB : forall (t : triple), t \in graph -> is_in_ib (subject t) == true
+                       ; predicate_in_I : forall (t : triple), t \in graph -> is_in_i (predicate t) == true
+                       ; object_in_IBL : forall (t : triple), t \in graph -> is_in_ibl (object t) == true
+                       }.
 
-  }.
+  Definition eqb_rdf (g1 g2 : rdf_graph) : bool :=
+    eqseq (graph g1) (graph g2).
+
+  Lemma graph_inj : forall (g1 g2: rdf_graph),
+      graph g1 == graph g2 ->
+      g1 = g2.
+  Proof. move=> [g1 sib1 pi1 oibl1] [g2 sib2 pi2 oibl2] /= /eqP geq.
+  Admitted.
+  
+
+  Definition rdf_eqP : Equality.axiom eqb_rdf.
+  Proof.
+    rewrite /Equality.axiom => x y.
+    apply: (iffP idP) => //= [| ->]; case: x y=> [g1 sib1 pi1 oibl1] [g2 sib2 pi2 oibl2]. move=> /eqP //= geq.
+    apply: graph_inj => //=. by rewrite geq eq_refl.
+    rewrite /eqb_rdf //=. elim g2 => [//|h t IHt]=> //=. rewrite eq_refl //=.
+  Qed.
 
 
-Definition image (g : rdf_graph) (μ : term -> term) : rdf_graph :=
-  mkRdfGraph (set_map eq_dec_triple (app_μ_to_triple μ) (graph g)).
+  Definition relabeling (g : rdf_graph) (μ : B -> B) : seq triple :=
+    map (fun t => relabeling t μ) (graph g).
 
-Definition eqb_graph (g g': rdf_graph) : bool :=
-  (match (set_diff eq_dec_triple (graph g) (graph g')) with
-   | nil => true
-   | otherwirse => false
-   end).
+  (* Definition eqb_graph (g g': rdf_graph) : bool := *)
+  (*   (match (set_diff eq_dec_triple (graph g) (graph g')) with *)
+  (*    | nil => true *)
+  (*    | otherwirse => false *)
+  (*    end). *)
 
-Inductive world : Type :=
-  | res (I L B : set term) (P : set_inter eq_dec_term I (set_inter eq_dec_term L B) = empty_set term).
+  (* Inductive world : Type := *)
+  (* | res (I L B : set term) (P : set_inter eq_dec_term I (set_inter eq_dec_term L B) = empty_set term). *)
 
-Definition proj_I (w : world) : set term :=
-  match w with
-  | res i _ _ _ => i
-  end.
-Definition proj_L (w : world) : set term :=
-  match w with
-  | res _ l _ _ => l
-  end.
+  (* Definition proj_I (w : world) : set term := *)
+  (*   match w with *)
+  (*   | res i _ _ _ => i *)
+  (*   end. *)
+  (* Definition proj_L (w : world) : set term := *)
+  (*   match w with *)
+  (*   | res _ l _ _ => l *)
+  (*   end. *)
 
-Definition proj_B (w : world) : set term :=
-  match w with
-  | res _ _ b _ => b
-  end.
-Definition proj_IL (w : world) : set term:=
-  set_union eq_dec_term (proj_I w) (proj_L w).
+  (* Definition proj_B (w : world) : set term := *)
+  (*   match w with *)
+  (*   | res _ _ b _ => b *)
+  (*   end. *)
+  (* Definition proj_IL (w : world) : set term:= *)
+  (*   set_union eq_dec_term (proj_I w) (proj_L w). *)
 
-Definition isomorphism (w : world) (g g': rdf_graph) :=
-  exists μ : term -> term,
-  relabelling (proj_IL w) (proj_B w) μ -> (image g μ) = g'.
+  (* Definition isomorphism (w : world) (g g': rdf_graph) := *)
+  (*   exists μ : term -> term, *)
+  (*     relabelling (proj_IL w) (proj_B w) μ -> (image g μ) = g'. *)
+
+End rdf.
 
