src/Triple.v
@@ -51,54 +51,23 @@ Section Triple.
 
   Canonical triple_eqType := EqType triple (EqMixin triple_eqP).
 
-  (* alias for triple of terms type *)
-  (* Definition triple := (node * term * term)%type.  *)
-
-(*
-    Inductive rdf : Type :=
-    | graph (triples : list triple).
- *)
-
-  (* Definition image (t : triple) (μ : B -> B) : triple := *)
-  (*   let (s,p,o,sin,pin,oin) := t in *)
-  (*   {μ s,μ p,μ o,sin,pin,oin}. *)
-
-
-
-
-  (* Definition eqb_triple (t1 t2:trpl) : bool := *)
-  (*   (match t1,t2 with *)
-  (*   | (triple s p o),(triple s2 p2 o2) => (eqb_term s s2) && (eqb_term p p2) && (eqb_term o o2) *)
-  (*   end). *)
-
-  (* Theorem eqb_eq_triple: forall (t1 t2 : trpl), *)
-  (*   eqb_triple t1 t2 = true <-> t1 = t2. *)
-  (* Proof. intros. split; intros H. *)
-  (*   - destruct t1,t2 as [s2 p2 o2]; f_equal; *)
-  (*     simpl in H; apply andb_true_iff in H; destruct H as [H0 H2]; apply andb_true_iff in H0; destruct H0 as [H H1]; apply eqb_eq_term.  *)
-  (*     + apply H. *)
-  (*     + apply H1. *)
-  (*     + apply H2. *)
-  (*   - destruct t1,t2 as [s2 p2 o2]. injection H as H1 H2 H3. simpl. rewrite H1. rewrite H2. rewrite H3. *)
-  (*     rewrite (eqb_term_refl s2). rewrite (eqb_term_refl p2). rewrite (eqb_term_refl o2). reflexivity. *)
-  (* Qed. *)
-
-  (* Theorem eqb_triple_refl : forall (t1: trpl), *)
-  (*   eqb_triple t1 t1 = true. *)
-  (* Proof. intros. destruct t1. simpl. rewrite (eqb_term_refl s). rewrite (eqb_term_refl p). rewrite (eqb_term_refl o). reflexivity. *)
-  (* Qed. *)
-
-  (* Theorem eqb_neq_triple : forall (t1 t2: trpl), *)
-  (*   eqb_triple t1 t2 = false <-> t1 <> t2. *)
-  (* Proof. intros. split. *)
-  (*   - intros H contra. rewrite contra in H. rewrite eqb_triple_refl in H. discriminate H. *)
-  (*   - intros H. unfold not in H. rewrite <- eqb_eq_triple in H. destruct (eqb_triple t1 t2). *)
-  (*     + exfalso. apply H. reflexivity. *)
-  (*     + reflexivity. *)
-  (* Qed. *)
-
-  (* Theorem eq_dec_triple : forall (t1 t2: trpl), *)
-  (*   {t1 = t2} + {t1 <> t2}. *)
-  (* Proof. decide equality; try decide equality; try apply string_dec; decide equality. Qed. *)
+  Lemma relabeling_preserves_is_in_ib : forall (t : term) (p: is_in_ib t == true) (μ : B -> B),
+      is_in_ib (relabeling t μ) == true.
+  Proof. move=> t. case t; by [].
+  Qed.
+  Lemma relabeling_preserves_is_in_i : forall (t : term) (p: is_in_i t == true) (μ : B -> B),
+      is_in_i (relabeling t μ) == true.
+  Proof. move=> t. case t; by [].
+  Qed.
+  Lemma relabeling_preserves_is_in_ibl : forall (t : term) (p: is_in_ibl t == true) (μ : B -> B),
+      is_in_ibl (relabeling t μ) == true.
+  Proof. move=> t. case t; by [].
+  Qed.
+  
+  Definition relabeling (t : triple) (μ : B -> B) : triple :=
+    let (s,p,o,sin,pin,oin) := t in
+    mkTriple (relabeling_preserves_is_in_ib sin μ)
+             (relabeling_preserves_is_in_i pin μ)
+             (relabeling_preserves_is_in_ibl oin μ).
 
 End Triple.
